$$
\prod_{k>0} 1/(1-x^k)^{a_k} = 1+x+2*\sum_{k>1} a_k x^k\dots两边Log\\
-\sum_{k>0}a_k\ln (1-x^k)=\ln (1+x+2\sum_{k>1}a_k x^k)\\
\sum_{k>0}(a_k\sum_{j>0}\frac{x^{jk}}{j})=\ln (1+x+2\sum_{k>1}a_k x^k)\\
\sum_{k>0}\sum_{j|k}(\frac{a_{k/j}}{j}x^{k})=\ln (1+x+2\sum_{k>1}a_k x^k)\\
\sum_{k>0}\sum_{j|k}(\frac{a_{j}}{k/j}x^{k})=\ln (1+x+2\sum_{k>1}a_k x^k)\\
\sum_{k>0}\sum_{j|k}(\frac{ja_{j}}{k}x^{k})=\ln (1+x+2\sum_{k>1}a_k x^k)\\
\sum_{k>0}\frac{x^k}{k}\sum_{j|k}ja_{j}=\ln (1+x+2\sum_{k>1}a_k x^k)\\
\sum_{k>0}x^k(a_k+\frac{1}{k}\sum_{j|k, j < k}ja_{j})=\ln (1+x+2\sum_{k>1}a_k x^k)\dots两边求导乘x
$$


$$
\sum_{k>0}x^k(ka_k+\sum_{j|k, j < k}ja_{j})=\frac{x+2\sum_{k>1}k a_k x^k}{1+x+2\sum_{k>1}a_k x^k}\\
\sum_{k>0}x^kka_k+\sum_{k>0}x^k\sum_{j|k, j < k}ja_{j}=\frac{x+2\sum_{k>1}k a_k x^k}{1+x+2\sum_{k>1}a_k x^k}\\
P(x)=\frac{-x+2R(x)}{1-x+2A(x)}\\
(1-x+2A(x))P(x)=-x+2R(x)\\
P(x)+(-x+2A(x))P(x)=-x+2R(x)\\
Q(x)+R(x)+(-x+2A(x))P(x)=-x+2R(x)\\
Q(x)+(-x+2A(x))P(x)+x=R(x)\\
$$
